examples/lowparse/LowParse.Spec.Seq.fst
@@ -13,7 +13,7 @@ val parse_seq_aux
   (#t: Type0)
   (p: bare_parser t)
   (b: bytes)
-: Tot (option (Seq.seq t * (consumed_length b)))
+: GTot (option (Seq.seq t * (consumed_length b)))
   (decreases (Seq.length b))
 
 let rec parse_seq_aux #t p b =
